tep_teq.v
@@ -3,6 +3,7 @@ Require Import TraceModel.
 Require Import Properties.
 Require Import CommonST.
 Require Import Robustdef.
+Require Import Criteria.
 Require Import Setoid.
 Require Import ClassicalExtras.
 Require Import Logic.ClassicalFacts.
@@ -70,4 +71,44 @@ Proof.
           inversion H1. congruence. now apply list_list_prefix_ref. 
        ++ apply (list_snoc_pointwise ll ll i2 i1 i1 i1) in H1; auto. 
           inversion H1. congruence. now apply list_list_prefix_ref.
+Qed.
+
+Definition RTIP :=
+  forall P1 P2,
+    (forall Cs, beh(Cs[P1]) ⊆ beh(Cs[P2])) -> 
+    (forall Ct, beh(Ct[P1↓]) ⊆ beh(Ct[P2↓])).
+
+
+Theorem R2RTP_RTIP : r2RPP -> RTIP.
+Proof.
+  intros r2rpp. unfold RTIP. apply NNPP.
+  intros hf. rewrite not_forall_ex_not in hf. destruct hf as [P1 hf].
+  rewrite not_forall_ex_not in hf. destruct hf as [P2 hf].
+  rewrite not_imp in hf. destruct hf as [H1 hf].
+  unfold "⊆" in *. 
+  rewrite not_forall_ex_not in hf. destruct hf as [Ct hf].
+  rewrite not_forall_ex_not in hf. destruct hf as [t hf].
+  rewrite not_imp in hf. destruct hf as [k1 k2].
+  specialize (r2rpp P1 P2 traces_match).
+  assert (Hsat : rsat2 P1 P2 traces_match).
+  { intros C b1 b2 Hb1 Hb2. apply (H1 C b1) in Hb1.
+    unfold beh in Hb1.         
+    now apply (determinacy_src (C [P2])). } 
+  specialize (r2rpp Hsat Ct t); clear Hsat.
+  assert (H : forall t2, sem tgt (Ct [P2 ↓]) t2 -> traces_match t t2). 
+  { intros t2 H. now apply r2rpp. } clear r2rpp H1.
+  destruct (longest_in_psem tgt_sem (Ct [P2 ↓]) t k2) as [l [Hmt [Hpsem_m Hmax_m]]].
+  destruct Hpsem_m as [t2 [Hmt2 Hsem_t2]].
+  specialize (H t2 Hsem_t2). destruct H; try now subst.
+  destruct H as [ll [i1 [i2 [Hi1 [Hi2 [Hdiffi [Hpref1 Hpref2]]]]]]].
+  assert (psem (Ct [P2 ↓]) (ftbd (snoc ll i1))).
+  { apply (input_totality_tgt (Ct [P2 ↓]) ll i2 i1); auto. now exists t2. }
+  assert (fpr (ftbd (snoc ll i1)) l) by now apply Hmax_m.
+  apply (fpr_pref_pref _ _ t2) in H0; auto.  
+  destruct (same_ext (ftbd (snoc ll i1)) (ftbd (snoc ll i2)) t2); auto;
+    simpl in H1.
+  ++ apply (list_snoc_pointwise ll ll i1 i2 i2 i2) in H1; auto. 
+     inversion H1. congruence. now apply list_list_prefix_ref. 
+  ++ apply (list_snoc_pointwise ll ll i2 i1 i1 i1) in H1; auto. 
+     inversion H1. congruence. now apply list_list_prefix_ref.
 Qed.
